---
title: "Tarea 2 (12-sept)"
---

## Ejercicio 1

$$
\begin{aligned}
-3x+2 &= -4 \\
-\frac{7}{4}-y &= -2x \\
\end{aligned} 
\implies
\left[
\begin{array}{cc|c}
-3 & 4 & -2 \\
2 & -1 & \frac{7}{4}
\end{array}
\right]
\\\\
$$

$$
\text{1) } F_1 = F_1+2F_2
$$

$$
\left[
\begin{array}{cc|c}
-3 & 4 & -2 \\
2 & -1 & \frac{7}{4}
\end{array}
\right]
\;\;\xrightarrow{F_1 = F_1+2F_2} \;\;
\left[
\begin{array}{cc|c}
1 & 2 & \frac{3}{2} \\
2 & -1 & \frac{7}{4}
\end{array}
\right]
\\\\
$$

$$
\text{2) } F_2 = F_2-2F_1
$$

$$
\left[
\begin{array}{cc|c}
1 & 2 & \frac{3}{2} \\
2 & -1 & \frac{7}{4}
\end{array}
\right]
\;\;\xrightarrow{F_2 = F_2-2F_1} \;\;
\left[
\begin{array}{cc|c}
1 & 2 & \frac{3}{2} \\
0 & -5 & -\frac{5}{4}
\end{array}
\right]
\\\\
$$

$$
\text{3) } F_2 = -\frac{1}{5}F_2
$$

$$
\left[
\begin{array}{cc|c}
1 & 2 & \frac{3}{2} \\
0 & -5 & -\frac{5}{4}
\end{array}
\right]
\;\;\xrightarrow{F_2 = -\frac{1}{5}F_2} \;\;
\left[
\begin{array}{cc|c}
1 & 2 & \frac{3}{2} \\
0 & 1 & \frac{1}{4}
\end{array}
\right]
\\\\
$$

$$
\text{4) } F_1 = F_1 -2F_2
$$

$$
\left[
\begin{array}{cc|c}
1 & 2 & \frac{3}{2} \\
0 & 1 & \frac{1}{4}
\end{array}
\right]
\;\;\xrightarrow{F_1 = F_1 -2F_2} \;\;
\left[
\begin{array}{cc|c}
1 & 0 & 1 \\
0 & 1 & \frac{1}{4}
\end{array}
\right]
\\\\
$$

### Solución
$$
\begin{aligned}
x &= 1 \\
y &= \frac{1}{4} \\
\end{aligned} 
$$


## Ejercicio 2

$$
\begin{align}
2x+y &= 5 \\
x-2y &= -5 \\
\end{align}
\implies
\left[
\begin{array}{cc|c}
2 & 1 & 5 \\
1 & -2 & -5
\end{array}
\right]
\\\\
$$

$$
\text{1) } F_1 \leftrightarrow F_2
$$

$$
\left[
\begin{array}{cc|c}
2 & 1 & 5 \\
1 & -2 & -5
\end{array}
\right]
\;\;\xrightarrow{F_1 \leftrightarrow F_2} \;\;
\left[
\begin{array}{cc|c}
1 & -2 & -5 \\
2 & 1 & 5
\end{array}
\right]
\\\\
$$

$$
\text{2) } F_2 = F_2-2F_1
$$

$$
\left[
\begin{array}{cc|c}
1 & -2 & -5 \\
2 & 1 & 5
\end{array}
\right]
\;\;\xrightarrow{F_2=F_2-2F_1} \;\;
\left[
\begin{array}{cc|c}
1 & -2 & -5 \\
0 & 5 & 15
\end{array}
\right]
\\\\
$$

$$
\text{3) } F_2 = \frac{1}{5}F_2
$$

$$
\left[
\begin{array}{cc|c}
1 & -2 & -5 \\
0 & 5 & 15
\end{array}
\right]
\;\;\xrightarrow{F_2 = \frac{1}{5}F_2} \;\;
\left[
\begin{array}{cc|c}
1 & -2 & -5 \\
0 & 1 & 3
\end{array}
\right]
\\\\
$$

$$
\text{4) } F_1 = F_1+2F_2
$$

$$
\left[
\begin{array}{cc|c}
1 & -2 & -5 \\
0 & 1 & 3
\end{array}
\right]
\;\;\xrightarrow{F_1 = F_1+2F_2} \;\;
\left[
\begin{array}{cc|c}
1 & 0 & 1 \\
0 & 1 & 3
\end{array}
\right]
\\\\
$$


### Solución
$$
\begin{aligned}
x &= 1 \\
y &= 3 \\
\end{aligned} 
$$


## Ejercicio 3

$$
\begin{align}
2x+3y+z &= 10 \\
x-y+2z &= 4 \\
3x+y-z &= 6
\end{align}
\implies
\left[
\begin{array}{ccc|c}
2 & 3 & 1 & 10 \\
1 & -1 & 2 & 4 \\
3 & 1 & -1 & 6 
\end{array}
\right]
\\\\
$$

$$
\text{1) } F_1 \leftrightarrow F_2
$$

$$
\left[
\begin{array}{ccc|c}
2 & 3 & 1 & 10 \\
1 & -1 & 2 & 4 \\
3 & 1 & -1 & 6 
\end{array}
\right]
\;\;\xrightarrow{F_1 \leftrightarrow F_2} \;\;
\left[
\begin{array}{ccc|c}
1 & -1 & 2 & 4 \\
2 & 3 & 1 & 10 \\
3 & 1 & -1 & 6 
\end{array}
\right]
\\\\
$$

$$
\text{2) } F_2 = F_2-2F_1
$$

$$
\left[
\begin{array}{ccc|c}
1 & -1 & 2 & 4 \\
2 & 3 & 1 & 10 \\
3 & 1 & -1 & 6 
\end{array}
\right]
\;\;\xrightarrow{F_2 = F_2-2F_1} \;\;
\left[
\begin{array}{ccc|c}
1 & -1 & 2 & 4 \\
0 & 5 & -3 & 2 \\
3 & 1 & -1 & 6 
\end{array}
\right]
\\\\
$$

$$
\text{3) } F_3 = F_3-3F_1
$$

$$
\left[
\begin{array}{ccc|c}
1 & -1 & 2 & 4 \\
0 & 5 & -3 & 2 \\
3 & 1 & -1 & 6  
\end{array}
\right]
\;\;\xrightarrow{F_3 = F_3-3F_1} \;\;
\left[
\begin{array}{ccc|c}
1 & -1 & 2 & 4 \\
0 & 5 & -3 & 2 \\
0 & 4 & -7 & -6 
\end{array}
\right]
\\\\
$$

$$
\text{4) } F_2 = \frac{1}{5}F_2
$$

$$
\left[
\begin{array}{ccc|c}
1 & -1 & 2 & 4 \\
0 & 5 & -3 & 2 \\
0 & 4 & -7 & -6 
\end{array}
\right]
\;\;\xrightarrow{F_2 = \frac{1}{5}F_2} \;\;
\left[
\begin{array}{ccc|c}
1 & -1 & 2 & 4 \\
0 & 1 & -\frac{3}{5} & \frac{2}{5} \\
0 & 4 & -7 & -6 
\end{array}
\right]
\\\\
$$

$$
\text{5) } F_3 = F_3-4F_2
$$

$$
\left[
\begin{array}{ccc|c}
1 & -1 & 2 & 4 \\
0 & 1 & -\frac{3}{5} & \frac{2}{5} \\
0 & 4 & -7 & -6 
\end{array}
\right]
\;\;\xrightarrow{F_3 = F_3-4F_2} \;\;
\left[
\begin{array}{ccc|c}
1 & -1 & 2 & 4 \\
0 & 1 & -\frac{3}{5} & \frac{2}{5} \\
0 & 0 & -\frac{23}{5} & -\frac{38}{5} 
\end{array}
\right]
\\\\
$$

$$
\text{6) } F_3 = -\frac{5}{23}F_3
$$

$$
\left[
\begin{array}{ccc|c}
1 & -1 & 2 & 4 \\
0 & 1 & -\frac{3}{5} & \frac{2}{5} \\
0 & 0 & -\frac{23}{5} & -\frac{38}{5} 
\end{array}
\right]
\;\;\xrightarrow{F_3 = -\frac{5}{23}F_3} \;\;
\left[
\begin{array}{ccc|c}
1 & -1 & 2 & 4 \\
0 & 1 & -\frac{3}{5} & \frac{2}{5} \\
0 & 0 & 1 & \frac{38}{23} 
\end{array}
\right]
\\\\
$$

$$
\text{7) } F_2 = F_2 +\frac{3}{5}F_3
$$

$$
\left[
\begin{array}{ccc|c}
1 & -1 & 2 & 4 \\
0 & 1 & -\frac{3}{5} & \frac{2}{5} \\
0 & 0 & 1 & \frac{38}{23} 
\end{array}
\right]
\;\;\xrightarrow{F_2 = F_2 +\frac{3}{5}F_3} \;\;
\left[
\begin{array}{ccc|c}
1 & -1 & 2 & 4 \\
0 & 1 & 0 & \frac{32}{23} \\
0 & 0 & 1 & \frac{38}{23} 
\end{array}
\right]
\\\\
$$

$$
\text{8) } F_1 = F_1 +F_2
$$

$$
\left[
\begin{array}{ccc|c}
1 & -1 & 2 & 4 \\
0 & 1 & 0 & \frac{32}{23} \\
0 & 0 & 1 & \frac{38}{23} 
\end{array}
\right]
\;\;\xrightarrow{F_1 = F_1 +F_2} \;\;
\left[
\begin{array}{ccc|c}
1 & 0 & 2 & \frac{124}{23} \\
0 & 1 & 0 & \frac{32}{23} \\
0 & 0 & 1 & \frac{38}{23} 
\end{array}
\right]
\\\\
$$

$$
\text{9) } F_1 = F_1-2F_3
$$

$$
\left[
\begin{array}{ccc|c}
1 & 0 & 2 & \frac{124}{23} \\
0 & 1 & 0 & \frac{32}{23} \\
0 & 0 & 1 & \frac{38}{23} 
\end{array}
\right]
\;\;\xrightarrow{F_1 = F_1-2F_3} \;\;
\left[
\begin{array}{ccc|c}
1 & 0 & 0 & \frac{48}{23} \\
0 & 1 & 0 & \frac{32}{23} \\
0 & 0 & 1 & \frac{38}{23} 
\end{array}
\right]
\\\\
$$

### Solución
$$
\begin{aligned}
x &= \frac{48}{23}  \\
y &= \frac{32}{23}  \\
z &= \frac{38}{23} 
\end{aligned} 
$$

## Ejercicio 4

$$
\begin{align}
2x+y-z &= 5 \\
-x+3y+2z &= 12 \\
4x-y+z &= 7
\end{align}
\implies
\left[
\begin{array}{ccc|c}
2 & 1 & -1 & 5 \\
-1 & 3 & 2 & 12 \\
4 & -1 & 1 & 7 
\end{array}
\right]
\\\\
$$

$$
\text{1) } F_1 \leftrightarrow F_2
$$

$$
\left[
\begin{array}{ccc|c}
2 & 1 & -1 & 5 \\
-1 & 3 & 2 & 12 \\
4 & -1 & 1 & 7 
\end{array}
\right]
\;\;\xrightarrow{F_1 \leftrightarrow F_2} \;\;
\left[
\begin{array}{ccc|c}
-1 & 3 & 2 & 12 \\
2 & 1 & -1 & 5 \\
4 & -1 & 1 & 7 
\end{array}
\right]
\\\\
$$

$$
\text{2) } F_1 =-F_1
$$

$$
\left[
\begin{array}{ccc|c}
-1 & 3 & 2 & 12 \\
2 & 1 & -1 & 5 \\
4 & -1 & 1 & 7 
\end{array}
\right]
\;\;\xrightarrow{F_1 =-F_1} \;\;
\left[
\begin{array}{ccc|c}
1 & -3 & -2 & -12 \\
2 & 1 & -1 & 5 \\
4 & -1 & 1 & 7 
\end{array}
\right]
\\\\
$$

$$
\text{3) } F_2 =F_2-2F_1
$$

$$
\left[
\begin{array}{ccc|c}
1 & -3 & -2 & -12 \\
2 & 1 & -1 & 5 \\
4 & -1 & 1 & 7 
\end{array}
\right]
\;\;\xrightarrow{F_2 =F_2-2F_1} \;\;
\left[
\begin{array}{ccc|c}
1 & -3 & -2 & -12 \\
0 & 7 & 3 & 29 \\
4 & -1 & 1 & 7 
\end{array}
\right]
\\\\
$$

$$
\text{4) } F_3 =F_3-4F_1
$$

$$
\left[
\begin{array}{ccc|c}
1 & -3 & -2 & -12 \\
0 & 7 & 3 & 29 \\
4 & -1 & 1 & 7 
\end{array}
\right]
\;\;\xrightarrow{F_3 =F_3-4F_1} \;\;
\left[
\begin{array}{ccc|c}
1 & -3 & -2 & -12 \\
0 & 7 & 3 & 29 \\
0 & 11 & 9 & 55 
\end{array}
\right]
\\\\
$$

$$
\text{5) } F_2 =\frac{1}{7}F_2
$$

$$
\left[
\begin{array}{ccc|c}
1 & -3 & -2 & -12 \\
0 & 7 & 3 & 29 \\
0 & 11 & 9 & 55  
\end{array}
\right]
\;\;\xrightarrow{F_2 =\frac{1}{7}F_2} \;\;
\left[
\begin{array}{ccc|c}
1 & -3 & -2 & -12 \\
0 & 1 & \frac{3}{7} & \frac{29}{7} \\
0 & 11 & 9 & 55 
\end{array}
\right]
\\\\
$$

$$
\text{6) } F_3 =F_3-11F_2
$$

$$
\left[
\begin{array}{ccc|c}
1 & -3 & -2 & -12 \\
0 & 1 & \frac{3}{7} & \frac{29}{7} \\
0 & 11 & 9 & 55 
\end{array}
\right]
\;\;\xrightarrow{F_3 =F_3-11F_2} \;\;
\left[
\begin{array}{ccc|c}
1 & -3 & -2 & -12 \\
0 & 1 & \frac{3}{7} & \frac{29}{7} \\
0 & 0 & \frac{30}{7} & \frac{66}{7} 
\end{array}
\right]
\\\\
$$

$$
\text{7) } F_3 =\frac{7}{30}F_3
$$

$$
\left[
\begin{array}{ccc|c}
1 & -3 & -2 & -12 \\
0 & 1 & \frac{3}{7} & \frac{29}{7} \\
0 & 0 & \frac{30}{7} & \frac{66}{7} 
\end{array}
\right]
\;\;\xrightarrow{F_3 =\frac{7}{30}F_3} \;\;
\left[
\begin{array}{ccc|c}
1 & -3 & -2 & -12 \\
0 & 1 & \frac{3}{7} & \frac{29}{7} \\
0 & 0 & 1 & \frac{11}{5} 
\end{array}
\right]
\\\\
$$

$$
\text{8) } F_2 =F_2-\frac{3}{7}F_3
$$

$$
\left[
\begin{array}{ccc|c}
1 & -3 & -2 & -12 \\
0 & 1 & \frac{3}{7} & \frac{29}{7} \\
0 & 0 & 1 & \frac{11}{5} 
\end{array}
\right]
\;\;\xrightarrow{F_2 =F_2-\frac{3}{7}F_3} \;\;
\left[
\begin{array}{ccc|c}
1 & -3 & -2 & -12 \\
0 & 1 & 0 & \frac{16}{5} \\
0 & 0 & 1 & \frac{11}{5} 
\end{array}
\right]
\\\\
$$

$$
\text{9) } F_1 =F_1+3F_2
$$

$$
\left[
\begin{array}{ccc|c}
1 & -3 & -2 & -12 \\
0 & 1 & 0 & \frac{16}{5} \\
0 & 0 & 1 & \frac{11}{5} 
\end{array}
\right]
\;\;\xrightarrow{F_1 =F_1+3F_2} \;\;
\left[
\begin{array}{ccc|c}
1 & 0 & -2 & -\frac{12}{5} \\
0 & 1 & 0 & \frac{16}{5} \\
0 & 0 & 1 & \frac{11}{5} 
\end{array}
\right]
\\\\
$$

$$
\text{10) } F_1 =F_1+2F_3
$$

$$
\left[
\begin{array}{ccc|c}
1 & 0 & -2 & -\frac{12}{5} \\
0 & 1 & 0 & \frac{16}{5} \\
0 & 0 & 1 & \frac{11}{5} 
\end{array}
\right]
\;\;\xrightarrow{F_1 =F_1+2F_3} \;\;
\left[
\begin{array}{ccc|c}
1 & 0 & 0 & 2 \\
0 & 1 & 0 & \frac{16}{5} \\
0 & 0 & 1 & \frac{11}{5} 
\end{array}
\right]
\\\\
$$

### Solución
$$
\begin{aligned}
x &= 2  \\
y &= \frac{16}{5}  \\
z &= \frac{11}{5} 
\end{aligned} 
$$


## Ejercicio 5

$$
\begin{align}
-2x+y &= \frac{1}{4} \\
-4x+4y &= 2
\end{align}
\implies
\left[
\begin{array}{cc|c}
-2 & 1 & \frac{1}{4} \\
-4 & 4 & 2
\end{array}
\right]
\\\\
$$

$$
\text{1) } F_1 \leftrightarrow F_2
$$

$$
\left[
\begin{array}{cc|c}
-2 & 1 & \frac{1}{4} \\
-4 & 4 & 2
\end{array}
\right]
\;\;\xrightarrow{F_1 \leftrightarrow F_2} \;\;
\left[
\begin{array}{cc|c}
-4 & 4 & 2 \\
-2 & 1 & \frac{1}{4}
\end{array}
\right]
\\\\
$$

$$
\text{2) } F_1 = -\frac{1}{4} F_1
$$

$$
\left[
\begin{array}{cc|c}
-4 & 4 & 2 \\
-2 & 1 & \frac{1}{4}
\end{array}
\right]
\;\;\xrightarrow{F_1 = -\frac{1}{4} F_1} \;\;
\left[
\begin{array}{cc|c}
1 & -1 & -\frac{2}{4} \\
-2 & 1 & \frac{1}{4}
\end{array}
\right]
\\\\
$$

$$
\text{3) } F_2 = F_2-2F_1
$$

$$
\left[
\begin{array}{cc|c}
1 & -1 & -\frac{2}{4} \\
-2 & 1 & \frac{1}{4}
\end{array}
\right]
\;\;\xrightarrow{F_2 = F_2-2F_1} \;\;
\left[
\begin{array}{cc|c}
1 & -1 & -\frac{2}{4} \\
0 & -1 & -\frac{3}{4}
\end{array}
\right]
\\\\
$$

$$
\text{4) } F_2 = -F_2
$$

$$
\left[
\begin{array}{cc|c}
1 & -1 & -\frac{2}{4} \\
0 & -1 & -\frac{3}{4}
\end{array}
\right]
\;\;\xrightarrow{F_2 = -F_2} \;\;
\left[
\begin{array}{cc|c}
1 & -1 & -\frac{2}{4} \\
0 & 1 & \frac{3}{4}
\end{array}
\right]
\\\\
$$

$$
\text{5) } F_1 = F_1+F_2
$$

$$
\left[
\begin{array}{cc|c}
1 & -1 & -\frac{2}{4} \\
0 & 1 & \frac{3}{4}
\end{array}
\right]
\;\;\xrightarrow{F_1 = -\frac{1}{4} F_1} \;\;
\left[
\begin{array}{cc|c}
1 & 0 & \frac{1}{4} \\
0 & 1 & \frac{3}{4}
\end{array}
\right]
\\\\
$$

### Solución
$$
\begin{aligned}
x &= \frac{1}{4} \\
y &= \frac{3}{4} \\
\end{aligned} 
$$

## Ejercicio 6

$$
\begin{align}
x+2y+\frac{3}{6}z &= 12 \\
2x+z &= 5+y \\
4x+8y+2z &= 2
\end{align}
\implies
\left[
\begin{array}{ccc|c}
1 & 2 & \frac{1}{2} & 12 \\
2 & -1 & 1 & 5 \\
4 & 8 & 2 & 2 
\end{array}
\right]
\\\\
$$

$$
\text{1) } F_3=F_3-4F_1
$$

$$
\left[
\begin{array}{ccc|c}
1 & 2 & \frac{1}{2} & 12 \\
2 & -1 & 1 & 5 \\
4 & 8 & 2 & 2 
\end{array}
\right]
\;\;\xrightarrow{F_3=F_3-4F_1} \;\;
\left[
\begin{array}{ccc|c}
1 & 2 & \frac{1}{2} & 12 \\
2 & -1 & 1 & 5 \\
0 & 0 & 0 & -46 
\end{array}
\right]
\\\\
$$

### Solución

El sistema no tiene solución pues el proceso da lugar a una inconsistencia: $0 = -46$